code/bignum/Hacl.Bignum.ModReduction.fst
@@ -1,0 +1,89 @@
+module Hacl.Bignum.ModReduction
+
+open FStar.HyperStack
+open FStar.HyperStack.ST
+open FStar.Mul
+
+open Lib.IntTypes
+open Lib.Buffer
+
+open Hacl.Bignum.Definitions
+
+module ST = FStar.HyperStack.ST
+module Loops = Lib.LoopCombinators
+module LSeq = Lib.Sequence
+module B = LowStar.Buffer
+
+module S = Hacl.Spec.Bignum.ModReduction
+module BN = Hacl.Bignum
+module BM = Hacl.Bignum.Montgomery
+
+#reset-options "--z3rlimit 50 --fuel 0 --ifuel 0"
+
+
+inline_for_extraction noextract
+let bn_mod_slow_precompr2_st (nLen:BN.meta_len) =
+    n:lbignum nLen
+  -> a:lbignum (nLen +! nLen)
+  -> r2:lbignum nLen
+  -> res:lbignum nLen ->
+  Stack unit
+  (requires fun h ->
+    live h n /\ live h a /\ live h r2 /\ live h res /\
+    disjoint res n /\ disjoint res a /\ disjoint res r2 /\ disjoint r2 n)
+  (ensures  fun h0 _ h1 -> modifies (loc res) h0 h1 /\
+    as_seq h1 res == S.bn_mod_slow_precompr2 (as_seq h0 n) (as_seq h0 a) (as_seq h0 r2))
+
+
+inline_for_extraction noextract
+val mk_bn_mod_slow_precompr2: nLen:BN.meta_len
+  -> (#[FStar.Tactics.Typeclasses.tcresolve ()] _ : Hacl.Bignum.Montgomery.mont nLen)
+  -> bn_mod_slow_precompr2_st nLen
+
+let mk_bn_mod_slow_precompr2 nLen #_ n a r2 res =
+  push_frame ();
+  let a_mod = create nLen (u64 0) in
+  let a1 = create (nLen +! nLen) (u64 0) in
+  copy a1 a;
+  let mu = BM.mod_inv_u64 n.(0ul) in
+  BM.reduction n mu a1 a_mod;
+  BM.to n mu r2 a_mod res;
+  pop_frame ()
+
+
+val bn_mod_slow_precompr2: nLen:BN.meta_len -> bn_mod_slow_precompr2_st nLen
+[@CInline]
+let bn_mod_slow_precompr2 nLen =
+  mk_bn_mod_slow_precompr2 nLen #(BM.mk_runtime_mont nLen)
+
+
+inline_for_extraction noextract
+let bn_mod_slow_st (nLen:BN.meta_len) =
+    n:lbignum nLen
+  -> a:lbignum (nLen +! nLen)
+  -> res:lbignum nLen ->
+  Stack unit
+  (requires fun h ->
+    live h n /\ live h a /\ live h res /\
+    disjoint res n /\ disjoint res a)
+  (ensures  fun h0 _ h1 -> modifies (loc res) h0 h1 /\
+    as_seq h1 res == S.bn_mod_slow (as_seq h0 n) (as_seq h0 a))
+
+
+inline_for_extraction noextract
+val mk_bn_mod_slow: nLen:BN.meta_len
+  -> (#[FStar.Tactics.Typeclasses.tcresolve ()] _ : Hacl.Bignum.Montgomery.mont nLen)
+  -> bn_mod_slow_st nLen
+
+let mk_bn_mod_slow nLen #k n a res =
+  push_frame ();
+  let r2 = create nLen (u64 0) in
+  BM.precomp 1ul n r2;
+  mk_bn_mod_slow_precompr2 nLen #k n a r2 res;
+  pop_frame ()
+
+
+val bn_mod_slow: nLen:BN.meta_len -> bn_mod_slow_st nLen
+[@CInline]
+let bn_mod_slow nLen =
+  mk_bn_mod_slow nLen #(BM.mk_runtime_mont nLen)
