code/bignum/Hacl.Spec.Bignum.ModReduction.fst
@@ -1,0 +1,89 @@
+module Hacl.Spec.Bignum.ModReduction
+
+open FStar.Mul
+
+open Lib.IntTypes
+open Lib.Sequence
+
+open Hacl.Spec.Bignum.Definitions
+
+module M = Hacl.Spec.Montgomery.Lemmas
+module BM = Hacl.Spec.Bignum.Montgomery
+module BI = Hacl.Spec.Bignum.ModInv64
+
+#reset-options "--z3rlimit 50 --fuel 0 --ifuel 0"
+
+///
+///  Modular reduction based on Montgomery arithmetic (it is slow!)
+///
+
+// TODO: we can pass a constant mu as well
+val bn_mod_slow_precompr2:
+    #nLen:size_pos{128 * nLen <= max_size_t}
+  -> n:lbignum nLen
+  -> a:lbignum (nLen + nLen)
+  -> r2:lbignum nLen ->
+  lbignum nLen
+
+let bn_mod_slow_precompr2 #nLen n a r2 =
+  let mu = BI.mod_inv_u64 n.[0] in
+  let a_mod = BM.mont_reduction n mu a in
+  let res = BM.to_mont n mu r2 a_mod in
+  res
+
+
+val bn_mod_slow_precompr2_lemma:
+    #nLen:size_pos{128 * nLen <= max_size_t}
+  -> n:lbignum nLen
+  -> a:lbignum (nLen + nLen)
+  -> r2:lbignum nLen -> Lemma
+  (requires
+    1 < bn_v n /\ bn_v n % 2 = 1 /\ bn_v a < bn_v n * bn_v n /\
+    bn_v r2 == pow2 (128 * nLen) % bn_v n)
+  (ensures bn_v (bn_mod_slow_precompr2 n a r2) == bn_v a % bn_v n)
+
+let bn_mod_slow_precompr2_lemma #nLen n a r2 =
+  let mu = BI.mod_inv_u64 n.[0] in
+  bn_eval_index n 0;
+  assert (bn_v n % pow2 64 == v n.[0]);
+  Math.Lemmas.pow2_modulo_modulo_lemma_1 (bn_v n) 2 64;
+  assert (v n.[0] % 2 = 1); // since bn_v n % 2 = 1
+  BI.mod_inv_u64_lemma n.[0];
+
+  let a_mod = BM.mont_reduction n mu a in
+  let res = BM.to_mont n mu r2 a_mod in
+  bn_eval_bound n nLen;
+  BM.mont_reduction_lemma n mu a;
+  BM.to_mont_lemma n mu r2 a_mod;
+
+  let d, k = M.eea_pow2_odd (64 * nLen) (bn_v n) in
+  M.mont_preconditions nLen (bn_v n) (v mu);
+  M.mont_reduction_lemma nLen (bn_v n) d (v mu) (bn_v a);
+  assert (bn_v a_mod == bn_v a * d % bn_v n);
+  M.to_mont_lemma nLen (bn_v n) d (v mu) (bn_v a_mod);
+  let r = pow2 (64 * nLen) in
+  assert (bn_v res == bn_v a_mod * r % bn_v n);
+  M.lemma_mont_id1 (bn_v n) r d (bn_v a);
+  assert (bn_v res == bn_v a % bn_v n)
+
+
+
+val bn_mod_slow:
+    #nLen:size_pos{128 * nLen <= max_size_t}
+  -> n:lbignum nLen
+  -> a:lbignum (nLen + nLen) ->
+  lbignum nLen
+
+let bn_mod_slow #nLen n a =
+  let r2 = BM.precomp_r2_mod_n 1 n in
+  bn_mod_slow_precompr2 #nLen n a r2
+
+
+val bn_mod_slow_lemma: #nLen:size_pos{128 * nLen <= max_size_t} -> n:lbignum nLen -> a:lbignum (nLen + nLen) -> Lemma
+  (requires 1 < bn_v n /\ bn_v n % 2 = 1 /\ bn_v a < bn_v n * bn_v n)
+  (ensures  bn_v (bn_mod_slow n a) == bn_v a % bn_v n)
+
+let bn_mod_slow_lemma #nLen n a =
+  let r2 = BM.precomp_r2_mod_n 1 n in
+  BM.precomp_r2_mod_n_lemma 1 n;
+  bn_mod_slow_precompr2_lemma #nLen n a r2
